keyset proved admitting properties of the RA

give-up.v
@@ -8,7 +8,7 @@ From iris.heap_lang Require Import proofmode notation par.
 From iris.bi.lib Require Import fractional.
 From iris.bi Require Import derived_laws_sbi.
 Set Default Proof Using "All".
-Require Export flows.
+Require Export flows keyset_ra.
 
 (* ---------- The program ---------- *)
 
@@ -20,7 +20,7 @@ Variable decisiveOp : (dOp → val).
 Variable searchStrSpec : (dOp → val).
 Variable lockLoc : node → loc.
 Variable getLockLoc : val.
-Variable keyset: node → gset key.
+Variable ks: node → gset key.
 
 Definition lockNode : val :=
   rec: "lockN" "x" :=
@@ -70,35 +70,29 @@ Definition nodesetΣ : gFunctors := #[GFunctor (authR (gsetUR node))].
 Instance subG_nodesetΣ {Σ} : subG nodesetΣ Σ → nodesetG Σ.
 Proof. solve_inG. Qed.
 
-(* RA for set of contents *)
-Class contentG Σ := ContentG { content_inG :> inG Σ (authR (gset_disjUR key)) }.
-Definition contentΣ : gFunctors := #[GFunctor (authR (gset_disjUR key))].
-
-Instance subG_contentΣ {Σ} : subG contentΣ Σ → contentG Σ.
-Proof. solve_inG. Qed.
-
-(* RA for keysets *)
-Class keysetG Σ := KeysetG { keyset_inG :> inG Σ (authR (gset_disjUR key)) }.
-Definition keysetΣ : gFunctors := #[GFunctor (authR (gset_disjUR key))].
+(* RA for pair of keysets and contents *)
+Class keysetG Σ := KeysetG { keyset_inG :> inG Σ (authUR (prodUR)) }.
+Definition keysetΣ : gFunctors := #[GFunctor (authUR (prodUR))].
 
 Instance subG_keysetΣ {Σ} : subG keysetΣ Σ → keysetG Σ.
 Proof. solve_inG. Qed.
 
 Section Give_Up_Template.
-  Context `{!heapG Σ, !flowintG Σ, !nodesetG Σ, !contentG Σ, !keysetG Σ} (N : namespace).
+  Context `{!heapG Σ, !flowintG Σ, !nodesetG Σ, !keysetG Σ} (N : namespace).
   Notation iProp := (iProp Σ).
 
 (* ---------- Flow interface set-up specific to this proof ---------- *)
 
   Variable root : node.
+  Variable KS : gset key.
   Variable hrep : node → flowintUR → gset key → iProp.
   Parameter hrep_timeless_proof : ∀ n I C, Timeless (hrep n I C).
   Instance hrep_timeless n I C: Timeless (hrep n I C).
   Proof. apply hrep_timeless_proof. Qed.
   Parameter hrep_fp : ∀ n I_n C, hrep n I_n C -∗ ⌜Nds I_n = {[n]}⌝.
   Parameter hrep_sep_star: ∀ n I_n I_n' C C', hrep n I_n C ∗ hrep n I_n' C' -∗ False.
-  Parameter keyset_disj: ∀ n n', n ≠ n' → keyset(n) ∩ keyset(n') = ∅.
-
+  Parameter KS_full : ∀ k, k ∈ KS.
+  
   Hypothesis globalint_root_fp: ∀ I, globalint I → root ∈ Nds I.
 
  (* Hypothesis globalint_fpo : ∀ I, globalint I → ∀ n:node, outf I n = 0.
@@ -107,38 +101,20 @@ Section Give_Up_Template.
   Hypothesis contextualLeq_impl_globalint :
     ∀ I I', globalint I →  contextualLeq I I' → globalint I'.
 
+  Hypothesis keyset_in_out : ∀ k In n, in_inset k In n → not_in_outset k In n → k ∈ ks n.
+  
   (* ---------- Coarse-grained specification ---------- *)
 
   Definition Ψ dop k (C: gset key) (C': gset key) (res: bool) : iProp :=
     match dop with
-    | memberOp => (⌜C' = C ∧ (Is_true res ↔ k ∈ C)⌝)%I
-    | insertOp => (⌜C' = union C {[k]} ∧ (Is_true res ↔ k ∉ C)⌝)%I
-    | deleteOp => (⌜C' = difference C {[k]} ∧ (Is_true res ↔ k ∈ C)⌝)%I
+    | memberOp => (⌜C' = C ∧ (if res then k ∈ C else k ∉ C)⌝)%I
+    | insertOp => (⌜C' = union C {[k]} ∧ (if res then k ∉ C else k ∈ C)⌝)%I
+    | deleteOp => (⌜C' = difference C {[k]} ∧ (if res then k ∈ C else k ∉ C)⌝)%I
     end.
 
   Instance Ψ_persistent dop k C C' res : Persistent (Ψ dop k C C' res).
   Proof. destruct dop; apply _. Qed.
 
-  Lemma Ψ_determines_res dop k C1 C1' C2 C2' res1 res2 :
-    Ψ dop k C1 C1' res1 ∗ Ψ dop k C2 C2' res2 ∗ ⌜C1 = C2⌝ -∗ ⌜res1 = res2⌝.
-  Proof.
-    destruct dop; iPureIntro; destr_bool;
-    destruct H as ((HC1 & HkC1) & (HC2 & HkC2) & HEq);
-    exfalso; rewrite HEq in HkC1; rewrite <- HkC2 in HkC1; inversion HkC1; contradiction.
-  Qed.
-
-  Lemma Ψ_determines_C' dop k C1 C1' C2 C2' res1 res2 :
-    Ψ dop k C1 C1' res1 ∗ Ψ dop k C2 C2' res2 ∗ ⌜C1 = C2⌝ -∗ ⌜C1' = C2'⌝.
-  Proof.
-    destruct dop; iPureIntro; simpl; destr_bool;
-    destruct H as ((HC1 & HkC1) & (HC2 & HkC2) & HEq); congruence.
-  Qed.
-(*
-  Axiom Ψ_keyset_theorem : ∀ (dop: dOp) (k: key) (n: node) (I_n I_n' I I': flowintUR) (res: bool),
-      ⌜globalint I⌝ ∗ ⌜Nds I_n = {[n]}⌝ ∗ ⌜in_inset k I_n n⌝ ∗ ⌜not_in_outset k I_n n⌝
-      ∗ ⌜(∃ (I_o: flowintUR), I = I_n ⋅ I_o ∧ I' = I_n' ⋅ I_o)⌝ ∗ ✓ I ∗ ✓ I'
-      -∗ Ψ dop k (cont I_n) (cont I_n') res -∗ ⌜Ψ dop k (cont I) (cont I') res⌝.
-*)
   (* ---------- Helper functions specs - proved for each implementation in GRASShopper ---------- *)
 
   Parameter getLockLoc_spec : ∀ (n: node),
@@ -167,31 +143,21 @@ Section Give_Up_Template.
        {{{ (b: bool) (I_n': flowintUR) (C': gset key) (res: bool),
                   RET (match b with false => NONEV | true => (SOMEV #res) end);
                   match b with false => hrep n I_n C |
-                              true => hrep n I_n' C' ∗ Ψ dop k C C' res ∗ ⌜ C' ⊆ keyset n⌝
+                              true => hrep n I_n' C' ∗ Ψ dop k C C' res ∗ ⌜ C' ⊆ ks n⌝
                                       ∗ ⌜contextualLeq I_n I_n'⌝ ∗ ⌜Nds I_n' = {[n]}⌝ end }}})%I.
 
   (* ---------- The invariant ---------- *)
 
-  Definition main_searchStr (γ γ_fp: gname) I Ns C
+  Definition main_searchStr (γ γ_fp γ_k : gname) I Ns (C: gset key)
     : iProp :=
-       ( own γ (● I) ∗ ⌜globalint I⌝
+       ( own γ_k (● prod (KS, C)) ∗ own γ (● I) ∗ ⌜globalint I⌝
         ∗ ([∗ set] n ∈ (Nds I), (∃ b: bool, (lockLoc n) ↦ #b ∗ if b then True
                                  else (∃ (In: flowintUR) (Cn: gset key), own γ (◯ In) ∗ hrep n In Cn 
-                                                                      ∗ ⌜Nds In = {[n]}⌝ ∗ ⌜keyset(n) ∩ C = Cn⌝ )))
+                                                ∗ ⌜Nds In = {[n]}⌝ ∗ own γ_k (◯ prod (ks(n), Cn)))))
         ∗ own γ_fp (● Ns) ∗ ⌜Ns = (Nds I)⌝
     )%I.
 
-  Definition is_searchStr γ γ_fp C := (∃ I Ns, (main_searchStr γ γ_fp I Ns C))%I.
-(*
-  Instance main_searchStr_timeless γ γ_fp γ_c I Ns C :
-    Timeless (main_searchStr γ γ_fp γ_c I Ns C).
-  Proof.
-    rewrite /main_searchStr. repeat apply bi.sep_timeless; try apply _.
-    try apply big_sepS_timeless. intros. apply bi.exist_timeless. intros.
-    apply bi.sep_timeless; try apply _.
-    destruct x0; try apply _.
-  Qed.
-*)
+  Definition is_searchStr γ γ_fp γ_k C := (∃ I Ns, (main_searchStr γ γ_fp γ_k I Ns C))%I.
 
   (* ---------- Assorted useful lemmas ---------- *)
 
@@ -215,6 +181,30 @@ Section Give_Up_Template.
     rewrite Hy in Hb. rewrite <- Ha in Hb. done.
   Qed.
 
+  Lemma auth_own_incl_ks γ x y : own γ (● x) ∗ own γ (◯ y) -∗ ⌜y ≼ x⌝.
+  Proof.
+    rewrite -own_op. rewrite own_valid. iIntros "Hown".
+    iEval (rewrite /(✓ (_)) /=) in "Hown".
+    iEval (rewrite /(cmra_op) /=) in "Hown".
+  Admitted.
+  
+  Lemma auth_ks_included (a1 a2 b1 b2: gset key) : prod (a1, b1) ≼ prod (a2, b2) 
+                → (a1 = a2 ∧ b1 = b2) ∨ 
+                    (∃ a0 b0, a2 = a1 ∪ a0 ∧ b2 = b1 ∪ b0 ∧ a1 ## a0 ∧ b1 ## b0 ∧ b1 ⊆ a1 ∧ b2 ⊆ a2 ∧ b0 ⊆ a0).
+  Proof.
+  Admitted.  
+  
+  Lemma auth_ks_local_update_insert K1 C Cn k: k ∈ K1 ∧ k ∉ Cn →
+             (prod (KS, C), prod (K1, Cn)) ~l~> (prod (KS, C ∪ {[k]}), prod (K1, Cn ∪ {[k]})).
+  Proof. 
+  Admitted.
+
+  Lemma auth_ks_local_update_delete K1 C Cn k: k ∈ K1 ∧ k ∈ Cn →
+             (prod (KS, C), prod (K1, Cn)) ~l~> (prod (KS, C ∖ {[k]}), prod (K1, Cn ∖ {[k]})).
+  Proof. 
+  Admitted.
+
+         
   Lemma flowint_update_result γ I I_n I_n' x :
     ⌜flowint_update_P I I_n I_n' x⌝ ∧ own γ x -∗
                        ∃ I', ⌜contextualLeq I I'⌝ ∗ ⌜∃ I_o, I = I_n ⋅ I_o ∧ I' = I_n' ⋅ I_o⌝
@@ -249,11 +239,11 @@ Section Give_Up_Template.
       iEval (rewrite Hd). iEval (rewrite <- H'). done.
   Qed.
 
-  Lemma inv_impl_fp n Ns γ γ_fp I Ns' C:
-    main_searchStr γ γ_fp I Ns' C ∗ own γ_fp (◯ Ns) ∗ ⌜n ∈ Ns⌝ -∗ ⌜n ∈ Nds I⌝.
+  Lemma inv_impl_fp n Ns γ γ_fp γ_k I Ns' C:
+    main_searchStr γ γ_fp γ_k I Ns' C ∗ own γ_fp (◯ Ns) ∗ ⌜n ∈ Ns⌝ -∗ ⌜n ∈ Nds I⌝.
   Proof.
     iIntros "(HInv & HNs & %)".
-    iDestruct "HInv" as "(? & ? & HIns & HNs' & %)".
+    iDestruct "HInv" as "(? & HIns & ? & ? & HNs' & %)".
     iPoseProof (auth_set_incl with "[$HNs $HNs']") as "%".
     iPureIntro. set_solver.
   Qed.                                       (* Made Proof using Type* *)
@@ -298,32 +288,18 @@ Section Give_Up_Template.
     iModIntro. done.
   Qed.
 
-
-  (* ---------- Ghost state manipulation to make final proof cleaner ---------- *)
-
-(*
-  Lemma ghost_update_root_fp γ γ_fp γ_c C:
-          is_searchStr γ γ_fp γ_c C ==∗
-                 ∃ (Ns: gsetUR node), is_searchStr γ γ_fp γ_c C ∗ own γ_fp (◯ Ns) ∗ ⌜root ∈ Ns⌝.
-  Proof.
-    iIntros "Hst". iModIntro.
-    iDestruct "Hst" as (I Ns) "(H1 & H2 & H3 & H4 & H5 & H6 & H7)".
-    iExists Ns.
-  Admitted.
-*)
-
   (* ---------- Refinement proofs ---------- *)
 
-  Lemma traverse_spec (γ γ_fp: gname) (k: key) (n: node) (Ns: gset node):
-       ⌜n ∈ Ns⌝ ∗ own γ_fp (◯ Ns) ∗ ⌜root ∈ Ns⌝ -∗ <<< ∀ C, is_searchStr γ γ_fp C >>>
+  Lemma traverse_spec (γ γ_fp γ_k: gname) (k: key) (n: node) (Ns: gset node):
+       ⌜n ∈ Ns⌝ ∗ own γ_fp (◯ Ns) ∗ ⌜root ∈ Ns⌝ -∗ <<< ∀ C, is_searchStr γ γ_fp γ_k C >>>
                 traverse root #n #k
                     @ ⊤
-          <<< ∃ (n': node) (Ns': gsetUR node) (I_n': flowintUR) (Cn: gset key), is_searchStr γ γ_fp C
-                      ∗ ⌜n' ∈ Ns'⌝ ∗ own γ_fp (◯ Ns') ∗ own γ (◯ I_n') ∗ hrep n' I_n' Cn
-                      ∗ ⌜Nds I_n' = {[n']}⌝ ∗ ⌜keyset(n') ∩ C = Cn⌝ ∗ ⌜in_inset k I_n' n'⌝ ∗ ⌜not_in_outset k I_n' n'⌝,
-                      RET #n' >>>.
-  Proof. Admitted.
-(*    iLöb as "IH" forall (n Ns). iIntros "(#Hinn & #Hfp & #Hroot)".
+          <<< ∃ (n': node) (Ns': gsetUR node) (I_n': flowintUR) (Cn: gset key), is_searchStr γ γ_fp γ_k C
+                      ∗ ⌜n' ∈ Ns'⌝ ∗ own γ_fp (◯ Ns') ∗ own γ (◯ I_n') ∗ hrep n' I_n' Cn 
+                      ∗ own γ_k (◯ prod (ks(n'), Cn)) ∗ ⌜Nds I_n' = {[n']}⌝ ∗ ⌜in_inset k I_n' n'⌝ 
+                      ∗ ⌜not_in_outset k I_n' n'⌝, RET #n' >>>.
+  Proof.
+    iLöb as "IH" forall (n Ns). iIntros "(#Hinn & #Hfp & #Hroot)".
     iIntros (Φ) "AU". wp_lam. wp_let. wp_bind(lockNode _)%E.
     awp_apply (lockNode_spec n). iApply (aacc_aupd_abort with "AU"); first done.
     iIntros (C0) "Hst". iDestruct "Hst" as (I Ns0)"(H2 & H3 & H4 & H5 & H6 & H7)".
@@ -331,13 +307,6 @@ Section Give_Up_Template.
     { iPoseProof ((auth_set_incl γ_fp Ns Ns0) with "[$]") as "%".
       iDestruct "H7" as %H7. iDestruct "Hinn" as %Hinn. iEval (rewrite <-H7).
       iPureIntro. set_solver. }
-    iAssert (⌜([^union set] n0 ∈ ({[n]} ∪ Nds I∖{[n]}), cont n0) ≡
-                ([^union set] n0 ∈ {[n]}, cont n0) ∪ ([^union set] n0 ∈ Nds I∖{[n]}, cont n0)⌝)%I with "[H2]" as "Hu".
-    { iDestruct "H2" as %H2. iPureIntro. apply leibniz_equiv_iff in H2.
-      apply (big_opS_union _ {[n]} (Nds I∖{[n]})). set_solver. }
-    assert ((Nds I) = ({[n]} ∪ (Nds I)∖ {[n]})) as Hn. { Check gset {[n]}. set_solver. }
-    iPoseProof (((big_opS_union) _ (Nds I∖{[n]}) {[n]}) with "[H2]") as "Hu".
-    { set_solver.
     rewrite (big_sepS_elem_of_acc _ (Nds I) n); last by eauto.
     iDestruct "H5" as "[Hb H5]".
     iDestruct "Hb" as (b) "[Hlock Hb]".
@@ -347,39 +316,39 @@ Section Give_Up_Template.
     destruct b. { iExFalso. done. } iModIntro.
     iSplitR "Hb". iExists I, Ns0. iFrame "∗ % #". iApply "H5". iExists true.
     iFrame. iIntros "AU". iModIntro. wp_pures.
-    iDestruct "Hb" as (In) "(HIn & Hrep & #HNds)". iDestruct "HNds" as %HNds.
-    wp_bind (inRange _ _)%E. wp_apply ((inRange_spec n In k) with "Hrep").
+    iDestruct "Hb" as (In Cn) "(HIn & Hrep & #HNds & HKS)". iDestruct "HNds" as %HNds.
+    wp_bind (inRange _ _)%E. wp_apply ((inRange_spec n In Cn k) with "Hrep").
     iIntros (b) "(Hrep & Hb)". destruct b.
     - wp_pures. wp_bind (findNext _ _)%E.
-      wp_apply ((findNext_spec n In k) with "Hrep").
+      wp_apply ((findNext_spec n In Cn k) with "Hrep").
       iIntros (b n') "(Hrep & Hbb)". destruct b.
       + wp_pures. awp_apply (unlockNode_spec n). 
         iApply (aacc_aupd_abort with "AU"); first done. iIntros (C1) "Hst".
-        iDestruct "Hst" as (I1 Ns1)"(H1 & H2 & H3 & H4 & H5 & H6 & H7)". 
-        iAssert (⌜n ∈ Nds I1⌝)%I with "[Hfp Hinn H6 H7]" as "%".
+        iDestruct "Hst" as (I1 Ns1)"(H1 & H2 & % & H5 & H6 & %)".
+        iAssert (⌜n ∈ Nds I1⌝)%I with "[Hfp Hinn H6]" as "%".
         { iPoseProof ((auth_set_incl γ_fp Ns Ns1) with "[$]") as "%".
-          iDestruct "H7" as %H7. iDestruct "Hinn" as %Hinn. iEval (rewrite <-H7).
+          iDestruct "Hinn" as %Hinn. iEval (rewrite <-H1).
           iPureIntro. set_solver. }
         rewrite (big_sepS_elem_of_acc _ (Nds I1) n); last by eauto.
         iDestruct "H5" as "[Hl H5]". iDestruct "Hl" as (b) "[Hlock Hl]".
-        destruct b; first last. { iDestruct "Hl" as (In') "(_ & Hrep' & _)".
+        destruct b; first last. { iDestruct "Hl" as (In' Cn') "(_ & Hrep' & _)".
         iAssert (⌜False⌝)%I with "[Hrep Hrep']" as %Hf. { iApply (hrep_sep_star n In In'). 
         iFrame. } exfalso. done. }
-        iAaccIntro with "Hlock". { iIntros "Hlock". iModIntro. iSplitR "HIn Hb Hrep Hbb".
+        iAaccIntro with "Hlock". { iIntros "Hlock". iModIntro. iSplitR "HIn HKS Hb Hrep Hbb".
         iExists I1, Ns1. iFrame "∗ % #". iApply "H5". iExists true. iFrame. iIntros "AU".
-        iModIntro. iFrame. } iIntros "Hlock". iDestruct "H7" as %H7.
-        iDestruct "Hb" as %Hb. iDestruct "Hbb" as %Hbb. iDestruct "H4" as %H4.
+        iModIntro. iFrame. } iIntros "Hlock".
+        iDestruct "Hb" as %Hb. iDestruct "Hbb" as %Hbb.
         iAssert (⌜n' ∈ Ns1⌝ ∗ ⌜root ∈ Ns1⌝ ∗ own γ (● I1) ∗ own γ_fp (● Ns1) ∗ own γ (◯ In))%I 
-                with "[HIn H3 H6]" as "Hghost".
+                with "[HIn H2 H6]" as "Hghost".
         { iPoseProof (auth_set_incl with "[$Hfp $H6]") as "%".
-          iPoseProof (auth_own_incl with "[$H3 $HIn]") as (I2)"%".
-          iPoseProof (own_valid with "H3") as "%".
+          iPoseProof (auth_own_incl with "[$H2 $HIn]") as (I2)"%".
+          iPoseProof (own_valid with "H2") as "%".
           iAssert (⌜n' ∈ Nds I1⌝)%I as "%".
           { iPureIntro. assert (n' ∈ Nds I2).
             { apply (flowint_step I1 In _ k n). done. 
               apply auth_auth_valid. done.
               replace (Nds In). set_solver. done. done. }
-            apply flowint_comp_fp in H2. set_solver. }
+            apply flowint_comp_fp in H4. set_solver. }
             iFrame. iPureIntro. replace Ns1. auto. }
         iDestruct "Hghost" as "(% & % & HAIn & HAfp & HIn)".
         iMod (own_update γ_fp (● Ns1) (● Ns1 ⋅ ◯ Ns1) with "HAfp") as "HNs".
@@ -389,49 +358,100 @@ Section Give_Up_Template.
         iFrame "∗ % #". iApply "H5". iExists false. iFrame. iExists In. eauto with iFrame.
         iIntros "AU". iModIntro. wp_pures. iApply "IH". iFrame "∗ % #". done.
       + iApply fupd_wp. iMod "AU" as (C) "[Hst [_ Hclose]]". iSpecialize ("Hclose" $! n Ns In).
-        iMod ("Hclose" with "[Hst HIn Hrep Hb Hbb]") as "HΦ".
-        iFrame "∗ % #". iModIntro.  wp_match. done.
+        iMod ("Hclose" with "[Hst HIn Hrep Hb Hbb HKS]") as "HΦ".
+        iFrame "∗ % #". iModIntro. wp_match. done.
     - wp_if. awp_apply (unlockNode_spec n). 
       iApply (aacc_aupd_abort with "AU"); first done. iIntros (C1) "Hst".
-      iDestruct "Hst" as (I1 Ns1)"(H1 & H2 & H3 & H4 & H5 & H6 & H7)". 
-      iAssert (⌜n ∈ Nds I1⌝)%I with "[Hfp Hinn H6 H7]" as "%".
+      iDestruct "Hst" as (I1 Ns1)"(H1 & H2 & % & H5 & H6 & %)".
+      iAssert (⌜n ∈ Nds I1⌝)%I with "[Hfp Hinn H6]" as "%".
       { iPoseProof ((auth_set_incl γ_fp Ns Ns1) with "[$]") as "%".
-        iDestruct "H7" as %H7. iDestruct "Hinn" as %Hinn. iEval (rewrite <-H7).
+        iDestruct "Hinn" as %Hinn. iEval (rewrite <-H1).
         iPureIntro. set_solver. }
       rewrite (big_sepS_elem_of_acc _ (Nds I1) n); last by eauto.
       iDestruct "H5" as "[Hl H5]". iDestruct "Hl" as (b) "[Hlock Hl]".
-      destruct b; first last. { iDestruct "Hl" as (In') "(_ & Hrep' & _)".
+      destruct b; first last. { iDestruct "Hl" as (In' Cn') "(_ & Hrep' & _)".
       iAssert (⌜False⌝)%I with "[Hrep Hrep']" as %Hf. { iApply (hrep_sep_star n In In'). 
       iFrame. } exfalso. done. }
-      iAaccIntro with "Hlock". { iIntros "Hlock". iModIntro. iSplitR "Hrep HIn".
+      iAaccIntro with "Hlock". { iIntros "Hlock". iModIntro. iSplitR "Hrep HIn HKS".
       iExists I1, Ns1. iFrame "∗ % #". iApply "H5". iExists true. iFrame. iIntros "AU".
       iModIntro. eauto with iFrame. } iIntros "Hlock". iModIntro.
       iSplitL. iExists I1, Ns1. iFrame "∗ % #". iApply "H5". iExists false. iFrame.
-      iExists In. eauto with iFrame. iIntros "AU". iModIntro. wp_pures.
+      iExists In, Cn. eauto with iFrame. iIntros "AU". iModIntro. wp_pures.
       iApply "IH". eauto with iFrame. done.
   Qed.
-*)
 
-  Theorem searchStrOp_spec (γ γ_fp : gname) (dop: dOp) (k: key):
-      <<< ∀ C, is_searchStr γ γ_fp C >>>
+
+  (* ---------- Ghost state manipulation to make final proof cleaner ---------- *)
+
+  Lemma ghost_update_keyset γ_k dop k Cn Cn' res K1 C:
+          Ψ dop k Cn Cn' res ∗ own γ_k (● prod (KS, C)) ∗ own γ_k (◯ prod (K1, Cn))
+                             ∗ ⌜Cn' ⊆ K1⌝ ∗ ⌜k ∈ K1⌝  ==∗
+                 ∃ C', Ψ dop k C C' res ∗ own γ_k (● prod (KS, C')) ∗ own γ_k (◯ prod (K1, Cn')).
+  Proof.
+    iIntros "(#HΨ & Ha & Hf & % & %)". iPoseProof (auth_own_incl_ks γ_k (prod (KS, C)) (prod (K1, Cn))
+                with "[$Ha $Hf]") as "%". apply (auth_ks_included _ _ _ _) in H1. destruct H1.
+    - iEval (unfold Ψ) in "HΨ". destruct H1. destruct dop. 
+      + iDestruct "HΨ" as "%". destruct H3.
+        iModIntro. iExists C. iEval (rewrite <-H3) in "Hf". iFrame. unfold Ψ.
+        iPureIntro. split; try done. rewrite <-H2. done.
+      + iDestruct "HΨ" as "%". destruct H3. destruct res.
+        * iMod (own_update_2 γ_k (● prod (KS, C)) (◯ prod (K1, Cn)) 
+          (● prod (KS, C ∪ {[k]}) ⋅ ◯ prod (K1, Cn ∪ {[k]})) with "[Ha] [Hf]") as "(Ha & Hf)"; try done.
+          { apply auth_update. apply auth_ks_local_update_insert. split; try done. }
+          iModIntro. iExists (C ∪ {[k]}). iEval (rewrite H3). iFrame.
+          unfold Ψ. iPureIntro. split; try done. rewrite <-H2. done.
+        * assert (Cn' = Cn). { set_solver. } iModIntro. iExists C. iEval (rewrite <-H5) in "Hf".
+          iFrame. unfold Ψ. iPureIntro. rewrite <- H2. split; try done. rewrite H5 in H3. done.
+      + iDestruct "HΨ" as "%". destruct H3. destruct res.
+        * iMod (own_update_2 γ_k (● prod (KS, C)) (◯ prod (K1, Cn)) 
+          (● prod (KS, C ∖ {[k]}) ⋅ ◯ prod (K1, Cn ∖ {[k]})) with "[Ha] [Hf]") as "(Ha & Hf)"; try done.
+          { apply auth_update. apply auth_ks_local_update_delete. split; try done. }
+          iModIntro. iExists (C ∖ {[k]}). iEval (rewrite H3). iFrame.
+          unfold Ψ. iPureIntro. split; try done. rewrite <-H2. done.
+        * assert (Cn' = Cn). { set_solver. } iModIntro. iExists C. iEval (rewrite <-H5) in "Hf".
+          iFrame. unfold Ψ. iPureIntro. rewrite <- H2. split; try done. rewrite H5 in H3. done.
+    - destruct H1 as [Ko [Co [H1 [H2 [H3 [H4 [H5 [H6 H7]]]]]]]]. destruct dop.
+      + iDestruct "HΨ" as "%". destruct H8.
+        iModIntro. iExists C. iEval (rewrite <-H8) in "Hf". iFrame. unfold Ψ.
+        iPureIntro. split; try done. destruct res; set_solver.
+      + iDestruct "HΨ" as "%". destruct H8. destruct res.
+        * iMod (own_update_2 γ_k (● prod (KS, C)) (◯ prod (K1, Cn)) 
+          (● prod (KS, C ∪ {[k]}) ⋅ ◯ prod (K1, Cn ∪ {[k]})) with "[Ha] [Hf]") as "(Ha & Hf)"; try done.
+          { apply auth_update. apply auth_ks_local_update_insert. split; try done. }
+          iModIntro. iExists (C ∪ {[k]}). iEval (rewrite H8). iFrame.
+          unfold Ψ. iPureIntro. split; try done. set_solver.
+        * assert (Cn' = Cn). { set_solver. } iModIntro. iExists C. iEval (rewrite <-H10) in "Hf".
+          iFrame. unfold Ψ. iPureIntro. set_solver.
+      + iDestruct "HΨ" as "%". destruct H8. destruct res.
+        * iMod (own_update_2 γ_k (● prod (KS, C)) (◯ prod (K1, Cn)) 
+          (● prod (KS, C ∖ {[k]}) ⋅ ◯ prod (K1, Cn ∖ {[k]})) with "[Ha] [Hf]") as "(Ha & Hf)"; try done.
+          { apply auth_update. apply auth_ks_local_update_delete. split; try done. }
+          iModIntro. iExists (C ∖ {[k]}). iEval (rewrite H8). iFrame.
+          unfold Ψ. iPureIntro. split; try done. set_solver.
+        * assert (Cn' = Cn). { set_solver. } iModIntro. iExists C. iEval (rewrite <-H10) in "Hf".
+          iFrame. unfold Ψ. iPureIntro. set_solver.
+  Qed.
+
+  Theorem searchStrOp_spec (γ γ_fp γ_k: gname) (dop: dOp) (k: key):
+      <<< ∀ C, is_searchStr γ γ_fp γ_k C >>>
             searchStrOp dop root #k
                   @ ⊤
-      <<< ∃ C' (res: bool), is_searchStr γ γ_fp C' 
-                                        ∗ ⌜Ψ dop k C C' res⌝, RET #res >>>.
+      <<< ∃ C' (res: bool), is_searchStr γ γ_fp γ_k C' 
+                                        ∗ Ψ dop k C C' res, RET #res >>>.
   Proof.
     iIntros (Φ) "AU". iLöb as "IH". wp_lam.
     iApply fupd_wp. iMod "AU" as (C0) "[Hst [HAU _]]".
-    iDestruct "Hst" as (I Ns0) "(H1 & % & H3 & H4 & %)".
+    iDestruct "Hst" as (I0 Ns0) "(H1 & H2 & % & H5 & H6 & %)".
     assert (root ∈ Ns0)%I as Hroot. { replace Ns0. apply globalint_root_fp. done. }
-    iMod (own_update γ_fp (● Ns0) (● Ns0 ⋅ ◯ Ns0) with "H4") as "HNs".
-    apply auth_update_core_id. apply gset_core_id. done. 
+    iMod (own_update γ_fp (● Ns0) (● Ns0 ⋅ ◯ Ns0) with "H6") as "HNs".
+    { apply auth_update_core_id. apply gset_core_id. done. } 
     iDestruct "HNs" as "(HAfp & #Hfp0)".
-    iMod ("HAU" with "[H1 H3 HAfp] ") as "AU". { iExists I, Ns0. iFrame "∗ % #". }
+    iMod ("HAU" with "[H1 H2 H5 HAfp] ") as "AU". { iExists I0, Ns0. iFrame "∗ % #". }
     iModIntro. wp_bind (traverse _ _ _)%E.
-    awp_apply (traverse_spec γ γ_fp k root Ns0). eauto with iFrame.
+    awp_apply (traverse_spec γ γ_fp γ_k k root Ns0). eauto with iFrame.
     iApply (aacc_aupd_abort with "AU"); first done.
     iIntros (C1) "Hst". iAaccIntro with "Hst"; first by eauto with iFrame.
-    iIntros (n Ns1 In Cn) "(Hst & #Hinn & #Hfp1 & HIn & Hrepn & #HNdsn & #Hkeyset & #Hinset & #Hnotout)".
+    iIntros (n Ns1 In Cn) "(Hst & #Hinn & #Hfp1 & HIn & Hrepn & HKS & #HNdsn & #Hinset & #Hnotout)".
     iModIntro. iFrame. iIntros "AU". iModIntro. wp_pures. wp_bind (decisiveOp _ _ _)%E.
     wp_apply ((decisiveOp_spec dop n k In Cn) with "[Hrepn]"). eauto with iFrame.
     iIntros (b In' Cn' res). iIntros "Hb". destruct b.
@@ -439,54 +459,51 @@ Section Give_Up_Template.
       wp_pures. wp_bind(unlockNode _)%E.
       awp_apply (unlockNode_spec n).
       iApply (aacc_aupd_commit with "AU"); first done. iIntros (C2) "Hst".
-      iDestruct "Hst" as (I1 Ns2)"(H1 & H2 & H3 & H4 & H5)". 
-      iAssert (⌜n ∈ Nds I1⌝)%I with "[Hfp1 Hinn H4 H5]" as "%".
+      iDestruct "Hst" as (I Ns2) "(H1 & H2 & % & H5 & H6 & %)".
+      iAssert (⌜n ∈ Nds I⌝)%I with "[Hfp1 Hinn H6]" as "%".
       { iPoseProof ((auth_set_incl γ_fp Ns1 Ns2) with "[$]") as "%".
-        iDestruct "H5" as %H5. iDestruct "Hinn" as %Hinn. iEval (rewrite <-H5).
+        iDestruct "Hinn" as %Hinn. iEval (rewrite <-H2).
         iPureIntro. set_solver. }
-      rewrite (big_sepS_elem_of_acc _ (Nds I1) n); last by eauto.
-      iDestruct "H3" as "[Hl H3]". iDestruct "Hl" as (b) "[Hlock Hl]".
+      rewrite (big_sepS_elem_of_acc _ (Nds I) n); last by eauto.
+      iDestruct "H5" as "[Hl H5]". iDestruct "Hl" as (b) "[Hlock Hl]".
       destruct b; first last. { iDestruct "Hl" as (In'' Cn'') "(_ & Hrep' & _)".
       iAssert (⌜False⌝)%I with "[Hrep Hrep']" as %Hf. { iApply (hrep_sep_star n In' In''). 
       iFrame. } exfalso. done. }
-      iAaccIntro with "Hlock". { iIntros "Hlock". iModIntro. iSplitR "HIn Hrep".
-      iExists I1, Ns2. iFrame "∗ % #". iApply "H3". iExists true.
-      iFrame. eauto with iFrame. }
-      iIntros "Hlock". iDestruct "H2" as %H2. iDestruct "H5" as %H5.
-(*       iDestruct "H2" as %H2. iEval (rewrite H2) in "H1". *)
-      iPoseProof (auth_own_incl with "[$H1 $HIn]") as (I2)"%".
-      iPoseProof ((own_valid γ (● I1)) with "H1") as "%". iDestruct "Hcon" as %Hcon.
-      iMod (own_updateP (flowint_update_P I1 In In') γ (● I1 ⋅ ◯ In) with "[H3 HIn]") as (?) "H0".
-      { apply (flowint_update I1 In In'). done. } { rewrite own_op. iFrame. }
-      iPoseProof ((flowint_update_result γ I1 In In') with "H0") as (I1') "(% & % & HIIn)".
-      iAssert (own γ (● I1') ∗ own γ (◯ In'))%I 
+      iAaccIntro with "Hlock". { iIntros "Hlock". iModIntro. iSplitR "HIn Hrep HKS".
+      iExists I, Ns2. iFrame "∗ % #". iApply "H5". iExists true. 
+      iFrame "Hlock". eauto with iFrame. } iIntros "Hlock".
+      iPoseProof (auth_own_incl with "[$H2 $HIn]") as (I2)"%".
+      iPoseProof ((own_valid γ (● I)) with "H2") as "%". iDestruct "Hcon" as %Hcon.
+      iMod (own_updateP (flowint_update_P I In In') γ (● I ⋅ ◯ In) with "[H2 HIn]") as (?) "H0".
+      { apply (flowint_update I In In'). done. } { rewrite own_op. iFrame. }
+      iPoseProof ((flowint_update_result γ I In In') with "H0") as (I') "(% & % & HIIn)".
+      iAssert (own γ (● I') ∗ own γ (◯ In'))%I 
                                 with "[HIIn]" as "(HI' & HIn')". { by rewrite own_op. }
-      iPoseProof ((own_valid γ (● I1')) with "HI'") as "%".
-      iPoseProof ((Ψ_keyset_theorem dop k n In In' I1 I1' res) 
-                                    with "[HNdsn Hinset Hnotout] [HΨ]") as "HΨI".
-      { repeat iSplitL; try done; iPureIntro; apply auth_auth_valid; done. } { done. }
-      iMod (own_update γ_c (cont I1) (cont I1') with "[H1]") as "H1'".
-      { apply (gset_update (cont I1) (cont I1')). } done.
-      iModIntro. iExists (cont I1'), res. iSplitL. iSplitR "HΨI".
-      { iExists I1', Ns2. assert (globalint I1') as HI'.
-      { apply (contextualLeq_impl_globalint I1 I1'). done. done. }
-      assert (Nds I1 = Nds I1') as HH. { apply (contextualLeq_impl_fp I1 I1'). done. }
-      iFrame "∗ % #". iSplitR. iPureIntro. reflexivity. iSplitL. iEval (rewrite HH) in "H5".
-      iApply "H5". iExists false. iFrame. iExists In'. eauto with iFrame. iPureIntro. set_solver. }
-      iEval (rewrite H2). done. iIntros "HΦ". iModIntro. wp_pures. done.
+      iPoseProof ((own_valid γ (● I')) with "HI'") as "%". iDestruct "Hsub" as "%".
+      iMod ((ghost_update_keyset γ_k dop k Cn Cn' res (ks n) C2) with "[H1 HKS]") as "Hgks".
+      iFrame "% ∗ #". iDestruct "Hinset" as %Hinset. iDestruct "Hnotout" as %Hnotout.
+      iPureIntro. apply (keyset_in_out k In n); try done. 
+      iDestruct "Hgks" as (C2') "(#HΨC & Ha & Hf)".
+      iModIntro. iExists (C2'), res. iSplitL. iSplitR "HΨC".
+      { iExists I', Ns2. assert (globalint I') as HI'.
+      { apply (contextualLeq_impl_globalint I I'). done. done. }
+      assert (Nds I = Nds I') as HH. { apply (contextualLeq_impl_fp I I'). done. }
+      rewrite HH in H2. iFrame "∗ % #". iEval (rewrite HH) in "H5".
+      iApply "H5". iExists false. iFrame. iExists In', Cn'. eauto with iFrame. } done.
+      iIntros "HΦ". iModIntro. wp_pures. done.
     - wp_match. awp_apply (unlockNode_spec n).
       iApply (aacc_aupd_abort with "AU"); first done. iIntros (C2) "Hst".
-      iDestruct "Hst" as (I1 Ns2)"(H1 & H2 & H3 & H4 & H5 & H6 & H7)". 
-      iAssert (⌜n ∈ Nds I1⌝)%I with "[Hfp1 Hinn H6 H7]" as "%".
+      iDestruct "Hst" as (I1 Ns2)"(H1 & H2 & % & H5 & H6 & %)". 
+      iAssert (⌜n ∈ Nds I1⌝)%I with "[Hfp1 Hinn H6]" as "%".
       { iPoseProof ((auth_set_incl γ_fp Ns1 Ns2) with "[$]") as "%".
-        iDestruct "H7" as %H7. iDestruct "Hinn" as %Hinn. iEval (rewrite <-H7).
+        iDestruct "Hinn" as %Hinn. iEval (rewrite <-H2).
         iPureIntro. set_solver. }
       rewrite (big_sepS_elem_of_acc _ (Nds I1) n); last by eauto.
       iDestruct "H5" as "[Hl H5]". iDestruct "Hl" as (b) "[Hlock Hl]".
-      destruct b; first last. { iDestruct "Hl" as (In'') "(_ & Hrep' & _)".
+      destruct b; first last. { iDestruct "Hl" as (In'' Cn'') "(_ & Hrep' & _)".
       iAssert (⌜False⌝)%I with "[Hb Hrep']" as %Hf. { iApply (hrep_sep_star n In In''). 
       iFrame. } exfalso. done. } iAaccIntro with "Hlock". { iIntros "Hlock". iModIntro.
-      iSplitR "HIn Hb". iExists I1, Ns2. iFrame "∗ % #". iApply "H5". iExists true. iFrame.
+      iSplitR "HIn Hb HKS". iExists I1, Ns2. iFrame "∗ % #". iApply "H5". iExists true. iFrame.
       eauto with iFrame. } iIntros "Hlock". iModIntro. iSplitL. iExists I1, Ns2. iFrame "∗ % #".
       iApply "H5". iExists false. eauto with iFrame. iIntros "AU". iModIntro.
       wp_pures. iApply "IH". done.
